problem 2 and 3 solved

Homework6.dfy
@@ -4,26 +4,41 @@ datatype List<T> = Nil | Cons(T, List<T>)
 
 function flatten<T>(tree:Tree<T>):List<T>
 ensures tree == Leaf ==> flatten(tree) == Nil
+decreases tree
 {
     match tree
         case Leaf => Nil
-        case Node(t1, t2, t) => append(Cons(t, flatten(t1)), flatten(t2))
+        case Node(l, r, t) => append(Cons(t, flatten(l)), flatten(r))
 }
 
 
 function append<T>(xs:List<T>, ys:List<T>):List<T>
+ensures xs == Nil ==> append(xs,ys) == ys
+ensures ys == Nil ==> append(xs,ys) == xs
+decreases xs
 {
-	
+	match xs
+        case Nil => ys
+        case Cons(x,xs') => Cons(x, append(xs',ys))
 }
 
 function treeContains<T>(tree:Tree<T>, element:T):bool
+ensures tree == Leaf ==> treeContains(tree, element) == false
+decreases tree
 {
-	
+	match tree
+        case Leaf => false
+        case Node(left, right, t) => t == element || treeContains(left, element) || treeContains(right, element)
 }
 
+
 function listContains<T>(xs:List<T>, element:T):bool
+ensures xs == Nil ==> listContains(xs, element) == false
+decreases xs
 {
-	
+	match xs
+        case Nil => false
+        case Cons(x, xs') => x == element || listContains(xs', element)
 }
 
 
